start.sh
@@ -1,0 +1,2 @@
+#! /bin/bash
+~/Isabelle2024/bin/isabelle jedit -d BridgeDefinition -l BridgeDefinition
